src/named/Core.v
@@ -6,12 +6,9 @@ Set Bullet Behavior "Strict Subproofs".
 
 From Utils Require Import Utils.
 From Named Require Import Exp Rule.
+Require Import String.
 
-Definition fresh {A} n (nl : named_list A) : bool :=
-  ~~ (n \in map fst nl).
-
-
-(* I want zip to be structural on s*)
+(* I want zip to be structural on s
 Definition zip' := 
 fun S T : Type =>
 fix zip (s : seq S) (t : seq T) {struct s} : seq (S * T) :=
@@ -29,7 +26,7 @@ Proof using .
   induction s; intro t; destruct t; simpl; f_equal; auto.
 Qed.
 
-(* TODO: which version?
+ TODO: which version?
 Definition with_names_from (c : ctx) (l : list exp) : subst :=
   (map (fun p => (fst (fst p), snd p)) (zip' c l)).
 
@@ -56,13 +53,16 @@ Transparent with_names_from.
 
 (* We could embed well-scopedness in bool, but well-typedness can be undecideable,
    so we leave it in Prop.
-   Expression constructors contain the level of the sort/term rule that proves them wf.
-   This is a deruijn level version of how Jon Sterling does it, but without symmetry
+   Expression constructors contain the name of the sort/term rule that proves them wf.
    
    For all judgments except wf_ctx and wf_lang,
    we assume the language and input context (where applicable) are well-formed.
 
+   For wf_args and wf_subst, we additionally assume the output context is well-formed.
+
    For the relational judgments, we assume all arguments are well-formed.
+   The relational judgments accept the items to be related last to play well
+   with tactics.
  *)
 Inductive le_sort (l : lang) c : sort -> sort -> Prop :=
 | le_sort_by : forall name t1 t2,
@@ -84,8 +84,6 @@ with le_term (l : lang) c : sort -> exp -> exp -> Prop :=
     le_subst l c c' s1 s2 ->
     le_term l c' t e1 e2 ->
     le_term l c t[/s2/] e1[/s1/] e2[/s2/]
-    (*choosing s1 would be a strictly stronger conclusion.
-      However, e2[/s2/] may not always have that type, so we must choose s2 *)
 | le_term_by : forall name t e1 e2,
     [:> !c |- (name) !e1 = !e2 : !t] \in l ->
     le_term l c t e1 e2
@@ -98,9 +96,9 @@ with le_term (l : lang) c : sort -> exp -> exp -> Prop :=
 | le_term_sym : forall t e1 e2, le_term l c t e1 e2 -> le_term l c t e2 e1
 (* Conversion:
 
-c |- e1 < e2 : t  ||
-               /\ ||
-c |- e1 < e2 : t' \/
+c |- e1 = e2 : t 
+               ||
+c |- e1 = e2 : t'
 *)
 | le_term_conv : forall t t',
     le_sort l c t t' ->
@@ -112,10 +110,8 @@ with le_subst (l : lang) c : ctx -> subst -> subst -> Prop :=
 | le_subst_cons : forall c' s1 s2,
     le_subst l c c' s1 s2 ->
     forall name t e1 e2,
-      fresh name c' ->
+      (* assumed because the output ctx is wf: fresh name c' ->*)
       le_term l c t[/s2/] e1 e2 ->
-    (*choosing s1 would be a strictly stronger premise,
-      this suffices since t[/s1/] <# t[/s2/] *)
     le_subst l c ((name, t)::c') ((name,e1)::s1) ((name,e2)::s2).
 
 Inductive le_args (l : lang) c : ctx -> list exp -> list exp -> Prop :=
@@ -123,27 +119,19 @@ Inductive le_args (l : lang) c : ctx -> list exp -> list exp -> Prop :=
 | le_args_cons : forall c' s1 s2,
     le_args l c c' s1 s2 ->
     forall name t e1 e2,
-      fresh name c' ->
+      (* assumed because the output ctx is wf: fresh name c' ->*)
       le_term l c t[/with_names_from c' s2/] e1 e2 ->
       le_args l c ((name, t)::c') (e1::s1) (e2::s2).
 
 
-Inductive wf_sort l c : sort -> Prop :=
-| wf_sort_by : forall n s c',
-    (n, (sort_rule c')) \in l ->
-    wf_args l c s c' ->
-    wf_sort l c (srt n s)
-with wf_term l c : exp -> sort -> Prop :=
+Inductive wf_term l c : exp -> sort -> Prop :=
 | wf_term_by : forall n s c' t,
     [:| !c' |- n : !t] \in l ->
     wf_args l c s c' ->
     wf_term l c (con n s) t[/(with_names_from c' s)/]
-(* terms can be lifted to greater (less precise) types,
-   but not the other way around; TODO: change the direction? might be more intuitive
- *)
 | wf_term_conv : forall e t t',
-    (* We add this condition so that we satisfy the assumptions of le_sort *)
-    wf_sort l c t' ->  
+    (* We add this condition so that we satisfy the assumptions of le_sort; todo: needed? 
+    wf_sort l c t' ->  *)
     wf_term l c e t ->
     le_sort l c t t' ->
     wf_term l c e t'
@@ -153,20 +141,24 @@ with wf_term l c : exp -> sort -> Prop :=
 with wf_args l c : list exp -> ctx -> Prop :=
 | wf_args_nil : wf_args l c [::] [::]
 | wf_args_cons : forall (s : list exp) c' name e t,
-    fresh name c' ->
+    (* assumed because the output ctx is wf: fresh name c' ->*)
     wf_args l c s c' ->
-    wf_sort l c' t ->
     wf_term l c e t[/with_names_from c' s/] ->
     wf_args l c (e::s) ((name,t)::c').
 
 Inductive wf_subst l c : subst -> ctx -> Prop :=
 | wf_subst_nil : wf_subst l c [::] [::]
 | wf_subst_cons : forall s c' name e t,
-    fresh name c' ->
+    (* assumed because the output ctx is wf: fresh name c' ->*)
     wf_subst l c s c' ->
-    wf_sort l c' t ->
     wf_term l c e t[/s/] ->
     wf_subst l c ((name,e)::s) ((name,t)::c').
+
+Variant wf_sort l c : sort -> Prop :=
+| wf_sort_by : forall n s c',
+    (n, (sort_rule c')) \in l ->
+    wf_args l c s c' ->
+    wf_sort l c (srt n s).
 
 Inductive wf_ctx l : ctx -> Prop :=
 | wf_ctx_nil : wf_ctx l [::]
@@ -176,7 +168,6 @@ Inductive wf_ctx l : ctx -> Prop :=
     wf_sort l c v ->
     wf_ctx l ((name,v)::c).
 
-Require Import String.
 
 Variant wf_rule l : rule -> Prop :=
 | wf_sort_rule : forall c,
@@ -204,6 +195,55 @@ Inductive wf_lang : lang -> Prop :=
     wf_lang l ->
     wf_rule l r ->
     wf_lang ((n,r)::l).
+
+(* build a database of presuppositions and judgment facts *)
+Create HintDb judgment discriminated.
+Hint Constructors wf_sort le_sort
+     wf_term le_term
+     wf_subst le_subst
+     wf_args le_args
+     wf_ctx wf_rule wf_lang : judgment.
+
+Scheme le_sort_ind' := Minimality for le_sort Sort Prop
+  with le_subst_ind' := Minimality for le_subst Sort Prop
+  with le_term_ind' := Minimality for le_term Sort Prop.
+
+Combined Scheme le_ind
+         from le_sort_ind', le_subst_ind', le_term_ind'.
+
+Scheme wf_args_ind' := Minimality for wf_args Sort Prop
+  with wf_term_ind' := Minimality for wf_term Sort Prop.
+
+Combined Scheme wf_ind
+         from wf_args_ind',
+         wf_term_ind'.
+
+Local Lemma wf_is_ws l c
+  : (forall s c', wf_args l c s c' -> well_scoped (map fst c) s)
+    /\ (forall e t, wf_term l c e t -> well_scoped (map fst c) e).
+Proof using .
+  eapply wf_ind; intros; simpl in *; break_goal; auto.
+  eapply pair_fst_in; eauto.
+Qed.    
+
+Definition wf_args_ws l c := proj1 (wf_is_ws l c).
+Hint Resolve wf_args_ws : judgment.
+Definition wf_term_ws l c := proj2 (wf_is_ws l c).
+Hint Resolve wf_term_ws : judgment.
+
+Lemma wf_sort_ws l c t : wf_sort l c t -> well_scoped (map fst c) t.
+Proof using .
+  inversion; simpl in *; eauto with judgment.
+Qed.
+Hint Resolve wf_sort_ws : judgment.
+
+Lemma wf_is_ws_ctx l c : wf_ctx l c -> ws_ctx c.
+Proof using .
+  elim: c; simpl; first by auto.
+  intro_to wf_ctx; inversion; apply /andP; split; [apply /andP|]; eauto with judgment.
+Qed.
+Hint Resolve wf_is_ws_ctx : judgment.
+
 
 Definition get_rule_ctx (r : rule) : ctx :=
   match r with
@@ -251,125 +291,10 @@ Qed.
 Lemma wf_term_var' n l c t :
     (n, t) \in c ->
     wf_term l c (var n) t.
-Proof.
+Proof using .
   constructor; assumption.
 Qed.
 
-  
-(* combines le_sort_by and le_sort_subst *)
-Lemma le_sort_refl' name l c : forall c' s1 s2,
-    [s| !c' |- name] \in l ->
-    len_eq s1 c' ->
-    len_eq s2 c' ->
-    le_args l c c' s1 s2 ->
-    le_sort l c (srt name s1) (srt name s2).
-Proof using .
-  intros.
-  repeat (match goal with [eqH : _ = _ |- _] => rewrite eqH; clear eqH end).
-Admitted  (*TODO:finish*).
-
-
-
-(* combines le_sort_by and le_sort_subst *)
-Lemma le_term_refl' name l c : forall c' s1 s2 t' t,
-    [:| !c' |- name : !t'] \in l ->
-    len_eq s1 c' ->
-    len_eq s2 c' ->
-    t = t'[/with_names_from c' s2/] ->
-    le_args l c c' s1 s2 ->
-    le_term l c t (con name s1) (con name s2).
-Proof using .
-  intros.
-  repeat (match goal with [eqH : _ = _ |- _] => rewrite eqH; clear eqH end).
-Admitted  (*TODO:finish*).
-
-(* combines le_sort_by and le_sort_subst *)
-Lemma le_sort_by' name l c : forall c' e1 e2 s1 s2 e1' e2',
-    [s> !c' |- (name) !e1 = !e2 ] \in l ->
-    len_eq s1 c' ->
-    len_eq s2 c' -> 
-    e1' = e1[/with_names_from c' s1/] ->
-    e2' = e2[/with_names_from c' s2/] ->
-    le_args l c c' s1 s2 ->
-    le_sort l c e1' e2'.
-Proof using .
-  intros.
-  repeat (match goal with [eqH : _ = _ |- _] => rewrite eqH; clear eqH end).
-  eapply le_sort_subst;[ | eapply le_sort_by; eassumption].
-Admitted  (*TODO:finish*).
-
-(* combines le_term_by and le_term_subst *)
-Lemma le_term_by' name l c : forall c' t e1 e2 s1 s2 t' e1' e2',
-    [:> !c' |- (name) !e1 = !e2 : !t] \in l ->
-    len_eq s1 c' ->
-    len_eq s2 c' ->                          
-    t' = t[/with_names_from c' s2/] ->
-    e1' = e1[/with_names_from c' s1/] ->
-    e2' = e2[/with_names_from c' s2/] ->
-    le_args l c c' s1 s2 ->
-    le_term l c t' e1' e2'.
-Proof using .
-  intros.
-  repeat (match goal with [eqH : _ = _ |- _] => rewrite eqH; clear eqH end).
-  eapply le_term_subst;[ | eapply le_term_by; eassumption].
-Admitted  (*TODO:finish*).
-
-Arguments le_term_by' name [l] {c} {c'} {t} {e1} {e2} {s1} {s2} {t'} {e1'} {e2'}.
-
-(* build a database of presuppositions and judgment facts *)
-Create HintDb judgment discriminated.
-Hint Constructors wf_sort le_sort
-     wf_term le_term
-     wf_subst le_subst
-     wf_args le_args
-     wf_ctx wf_rule wf_lang : judgment.
-
-(* monotonicity of judgments under language extension *)
-
-
-Scheme le_sort_ind' := Minimality for le_sort Sort Prop
-  with le_subst_ind' := Minimality for le_subst Sort Prop
-  with le_term_ind' := Minimality for le_term Sort Prop.
-
-Combined Scheme le_ind
-         from le_sort_ind', le_subst_ind', le_term_ind'.
-
-Scheme wf_sort_ind' := Minimality for wf_sort Sort Prop
-  with wf_args_ind' := Minimality for wf_args Sort Prop
-  with wf_term_ind' := Minimality for wf_term Sort Prop.
-
-Combined Scheme wf_ind
-         from wf_sort_ind',
-         wf_args_ind',
-         wf_term_ind'.
-
-(*TODO: needed?
-Ltac expand_rule_shift :=
-  match goal with
-  | |- context [ {| ?c ::%! 1 |- sort}] =>
-    change ({| ?c ::%! 1 |- sort})
-      with ({| c |- sort})%%!1
-  | |- context [ {| ?c ::%! 1 |- ?t %! 1}] =>
-    change ({| ?c ::%! 1 |- ?t %! 1})
-      with ({| c |- t})%%!1
-  | |- context [ {<?c1 ::%! 1 <# ?c2 ::%! 1 |- ?t1 %! 1 <# ?t2 %! 1}] =>
-    change ({<?c1 ::%! 1 <# ?c2 ::%! 1 |- ?t1 %! 1 <# ?t2 %! 1})
-      with ({<c1 <# c2 |- t1 <# t2})%%!1
-  | |- context [ {<?c1 ::%! 1 <# ?c2 ::%! 1 |- ?e1%!1 <# ?e2%!1 .: ?t1 %! 1 <# ?t2 %! 1}] =>
-    change ({<?c1 ::%! 1 <# ?c2 ::%! 1 |- ?e1%!1 <# ?e2%!1 .: ?t1 %! 1 <# ?t2 %! 1})
-      with ({<c1 <# c2 |- e1 <# e2 .: t1 <# t2})%%!1
-  end. *)
-
-(* TOOD: do I need a named analogue? 
-Lemma is_nth_level_cons {A : eqType} l n t (r : A) : is_nth_level l n t -> is_nth_level (r::l) n t.
-Proof using .  
-  unfold is_nth_level.
-  move /andP => [nlts] /eqP <-.
-  simpl.
-  apply /andP; split.
-  auto.
-  rewrite subSn; auto.
-Qed.*)
 
 Lemma wf_subst_len_eq l c s c' : wf_subst l c s c' -> size s = size c'.
 Proof using .
@@ -403,45 +328,7 @@ Proof using .
 Qed.
 
 
-(* TODO: do I need a named analogue?
-Lemma nth_level_size_lt {A:eqType} l n e : @is_nth_level A l n e -> n < size l.
-Proof using .
-  unfold is_nth_level.
-  move /andP; tauto.
-Qed.
-*)
-
-(* TODO: wsness with names
-Lemma wf_is_ws l c
-  : (forall t, wf_sort l c t -> ws_exp (size c) t)
-    /\ (forall s c', wf_subst l c s c' -> ws_subst (size c) s)
-    /\ (forall e t, wf_term l c e t -> ws_exp (size c) e).
-Proof using .
-  Scheme t_ind := Minimality for wf_sort Sort Prop
-  with s_ind := Minimality for wf_subst Sort Prop
-  with e_ind := Minimality for wf_term Sort Prop.
-
-  Combined Scheme ind from t_ind, s_ind, e_ind.
-  move: c;
-  apply: ind; simpl; intros;
-  try apply /andP; auto; try apply: nth_level_size_lt; eauto.
-Qed.
-Definition wf_is_ws_sort l c := proj1 (wf_is_ws l c).
-Hint Resolve wf_is_ws_sort : judgment.
-
-Definition wf_is_ws_subst l c := proj1 (proj2 (wf_is_ws l c)).
-Hint Resolve wf_is_ws_subst : judgment.
-
-Definition wf_is_ws_term l c := proj2 (proj2 (wf_is_ws l c)).
-Hint Resolve wf_is_ws_term : judgment.
-
-Lemma wf_is_ws_ctx l c : wf_ctx l c -> ws_ctx c.
-Proof.
-  elim: c; simpl; first by auto.
-  intro_to wf_ctx; inversion; apply /andP; eauto with judgment.
-Qed.
-Hint Resolve wf_is_ws_ctx : judgment.
-
+(* TODO
 Lemma wf_is_ws_rule l r : wf_rule l r -> ws_rule r.
 Proof.
   case: r; intro_to wf_rule; inversion; simpl.
@@ -458,22 +345,61 @@ Proof using .
 Qed.
 Hint Resolve le_subst_refl : judgment.
 
+Lemma wf_subst_names_eq l c s c'
+  : wf_subst l c s c' -> map fst s = map fst c'.
+Proof using .
+  elim; intros; simpl in *; eauto.
+  f_equal; auto.
+Qed.
+Hint Resolve wf_subst_names_eq : judgment.
 
+Lemma le_subst_names_eq_l l c c' s1 s2
+  : le_subst l c c' s1 s2 -> map fst s1 = map fst c'.
+Proof using .
+  elim; intros; simpl in *; eauto.
+  f_equal; auto.
+Qed.
+Hint Resolve le_subst_names_eq_l : judgment.
+
+
+Lemma le_subst_names_eq_r l c c' s1 s2
+  : le_subst l c c' s1 s2 -> map fst s2 = map fst c'.
+Proof using .
+  elim; intros; simpl in *; eauto.
+  f_equal; auto.
+Qed.
+Hint Resolve le_subst_names_eq_r : judgment.
+
+(*
 Lemma lookup_wf l c d (n : string) t c' s
   : wf_ctx l c -> (n, t) \in c ->
     wf_subst l c' s c -> wf_term l c' (named_list_lookup d s n) t [/s /].
 Proof.
-  elim: c n; simpl.
-  intros n _.
-  inversion.
+  elim: c s n; simpl.
+  intros s n _; inversion.
   intro_to wf_ctx; inversion; subst.
   rewrite in_cons.
-  case heq: ((n,t) == (name,v)); simpl.
+  case neq:(n==name); simpl.
+  case teq: (t == v); simpl.
   {
-    move: heq => /eqP <- _.
+    move: neq teq => /eqP neq /eqP teq.
+    rewrite -!neq -!teq.
+    rewrite eq_refl;simpl.
+    intro.
     inversion; subst.
     simpl.
-    replace (n=?n)%string with true.
+    rewrite eqb_refl.
+    change (sort_subst ?s v) with v[/s/].
+    rewrite ws_sort_mono; auto.
+    erewrite fresh_iff_names_eq; eauto using wf_subst_names_eq.
+    erewrite  wf_subst_names_eq; eauto with judgment.
+  }
+  {
+    change ((n,t)==(name,v)) with ((n==name)&&(t==v)).
+    rewrite teq neq; simpl.
+    
+    move: 
+    
   (*  TODO: use wsness
   case: n; simpl.
   intro.
@@ -487,7 +413,7 @@ Proof.
 
   Fail.*)*)
 Admitted.
-
+*)
 (*
 Lemma rule_in_ws l r : wf_lang l -> r \in l -> ws_rule r.
 Proof using .
@@ -507,40 +433,76 @@ Lemma mono_le_subst l c
         forall c' s1 s2, le_subst l c' c s1 s2 ->
                          le_sort l c' t1[/s1/] t2[/s2/])
     /\ (forall c' s1 s2,
-           le_subst l c c' s1 s2 -> wf_ctx l c' ->
+           le_subst l c c' s1 s2 -> ws_ctx c' ->
            forall c'' s1' s2', le_subst l c'' c s1' s2' ->
-                               le_subst l c'' c' (subst_cmp s1 s1') (subst_cmp s2 s2'))
+                               le_subst l c'' c' s1[/s1'/] s2[/s2'/])
     /\ (forall t e1 e2,
-           le_term l c t e1 e2 ->
+           le_term l c t e1 e2 -> well_scoped (map fst c) t ->
            forall c' s1 s2, le_subst l c' c s1 s2 ->
                             le_term l c' t[/s2/] e1[/s1/] e2[/s2/]).
 Proof with eauto with judgment using.
-  (*
-  move: c; apply: le_ind; intros; simpl...
-  move: H3; simpl; move /andP => [wst wsc].
-  constructor...
-  (*TODO: this step is automatable*)
-  rewrite sep_subst_cmp...
-  (*TODO: this step is automatable*)
-  erewrite le_subst_len_eq_r...
-Qed.*)
-Admitted.
+  move: c; apply: le_ind; intros; break; simpl in *; break...
+  constructor; fold_Substable...
+  rewrite <-subst_assoc...
+  erewrite le_subst_names_eq_r...
+Qed.
 
+
+Lemma with_names_from_args_subst c' s' s
+  : with_names_from c' (args_subst s' s) = (with_names_from c' s)[/s'/].
+Proof using .
+  elim: c' s; intros until s; case: s; intros; break; simpl in *; auto.
+  f_equal; auto.
+  by fold_Substable.
+Qed.
+
+Lemma map_fst_with_names_from c s
+  : size s = size c -> map fst (with_names_from c s) = map fst c.
+Proof using .
+  elim: c s; intros until s; case: s; intros; break;simpl in *; auto.
+  { inversion H0. }
+  {
+    f_equal; auto.
+  }
+Qed.
+  
 Lemma mono_wf_subst l c
   : wf_lang l (*TODO: just used for wsness; handle differently? ws syntax?*)->
-    (forall t,
-           wf_sort l c t -> wf_ctx l c ->
-           forall c' s, wf_subst l c' s c ->
-                        wf_sort l c' t[/s/])
-    /\ (forall s c',
-           wf_subst l c s c' -> wf_ctx l c ->
+    (forall s c',
+           wf_args l c s c' ->
+           wf_ctx l c ->
+           ws_ctx c' ->
            forall c'' s', wf_subst l c'' s' c ->
-                          wf_subst l c'' (subst_cmp s s') c')
+                          wf_args l c'' s[/s'/] c')
     /\ (forall e t,
-           wf_term l c e t -> wf_ctx l c ->
+           wf_term l c e t ->
+           wf_ctx l c ->
+           well_scoped (map fst c) t ->
            forall c' s, wf_subst l c' s c ->
                         wf_term l c' e[/s/] t[/s/]).
 Proof with eauto with judgment using .
+  move => wfl; apply wf_ind; intros; simpl in *; break_andbs...
+  {
+    econstructor...
+    rewrite with_names_from_args_subst.
+    rewrite -subst_assoc...
+    {
+      apply H2...
+      change (sort_subst ?s ?t) with t[/s/].
+      apply ws_sort_subst.
+      rewrite ws_subst_args.
+      break_goal...
+      Search _ ws_subst.
+      TODO: ws sub from ws args
+    rewrite map_fst_with_names_from...
+    Search _ (map fst (with_names_from _ _)).
+
+
+    Lemma mono_subst_wf_sort: (forall t,
+           wf_sort l c t -> wf_ctx l c ->
+           forall c' s, wf_subst l c' s c ->
+                        wf_sort l c' t[/s/])
+    /\ 
 (*
   move => wfl; move:c; apply wf_ind; intros; simpl; try by econstructor; eauto with judgment.
   { (* wf_term_subst *)
@@ -585,12 +547,6 @@ Hint Resolve mono_subst_wf_subst : judgment.
 Definition mono_subst_wf_term l c wfl :=
   proj2 (proj2 (@mono_wf_subst l c wfl)).
 Hint Resolve mono_subst_wf_term : judgment.
-
-Lemma wf_subst_ctx l c s c' : wf_subst l c s c' -> wf_ctx l c'.
-Proof.
-  elim; eauto with judgment.
-Qed.
-Hint Resolve wf_subst_ctx :judgment.
 
 
 Lemma mono_ext_le l n r c
@@ -1315,3 +1271,119 @@ Ltac wf_to_ctx_from_rule :=
   inversion H.
 *)
 *)
+
+
+
+(* TODO: all_fresh is harder to satisfy than I thought; needs wf_lang, or sim.
+   not a problem, but needs work to do*)
+Lemma unsubst_id_sort n s c
+  : all_fresh c -> len_eq s c -> (srt n s) = (srt n (map var (map fst c)))[/with_names_from c s/].
+Proof.
+  elim: s c; intros until c; case: c.
+  all: repeat match goal with
+  | [|- forall _:(_*_),_] => case; intro; intro
+  | [|- forall _:seq _,_] => intro
+  | [|- is_true (all_fresh (_::_)) -> _] => simpl; move /andP; case
+  | [|- is_true (all_fresh _) -> _] => intro
+  | [|- is_true (fresh _ _) -> _] => intro
+  | [|- len_eq _ _ -> _] => first [ by inversion | intro ]
+  end.  
+  simpl.
+  f_equal.
+  f_equal.
+  {
+    cbn.
+    rewrite eqb_refl.
+    reflexivity.
+  }
+  {
+    simpl in H.
+    inversion H0; subst.
+    specialize (H l0 b0 H2).
+    move: H.
+    case.
+    move ->.
+    admit (*TODO fresh var doesn't affect subst*).
+  }
+Admitted.
+
+(* combines le_sort_by and le_sort_subst *)
+Lemma le_sort_refl' name l c : forall c' s1 s2,
+    wf_lang l ->
+    [s| !c' |- name] \in l ->
+    len_eq s1 c' ->
+    len_eq s2 c' ->
+    le_args l c c' s1 s2 ->
+    le_sort l c (srt name s1) (srt name s2).
+Proof using .
+  intros.
+  erewrite unsubst_id_sort; eauto.
+  replace (srt name s2) with (srt name (map var (map fst c')))[/with_names_from c' s2/];
+    [| erewrite <-unsubst_id_sort; eauto].
+  eapply le_sort_subst.
+  eapply le_args_le_subst.
+  constructor.
+  eauto with judgment.
+  
+  repeat (match goal with [eqH : _ = _ |- _] => rewrite eqH; clear eqH end).
+Admitted  (*TODO:finish*).
+
+
+
+(* combines le_sort_by and le_sort_subst *)
+Lemma le_term_refl' name l c : forall c' s1 s2 t' t,
+    [:| !c' |- name : !t'] \in l ->
+    len_eq s1 c' ->
+    len_eq s2 c' ->
+    t = t'[/with_names_from c' s2/] ->
+    le_args l c c' s1 s2 ->
+    le_term l c t (con name s1) (con name s2).
+Proof using .
+  intros.
+  repeat (match goal with [eqH : _ = _ |- _] => rewrite eqH; clear eqH end).
+Admitted  (*TODO:finish*).
+
+(* combines le_sort_by and le_sort_subst *)
+Lemma le_sort_by' name l c : forall c' e1 e2 s1 s2 e1' e2',
+    [s> !c' |- (name) !e1 = !e2 ] \in l ->
+    len_eq s1 c' ->
+    len_eq s2 c' -> 
+    e1' = e1[/with_names_from c' s1/] ->
+    e2' = e2[/with_names_from c' s2/] ->
+    le_args l c c' s1 s2 ->
+    le_sort l c e1' e2'.
+Proof using .
+  intros.
+  repeat (match goal with [eqH : _ = _ |- _] => rewrite eqH; clear eqH end).
+  eapply le_sort_subst;[ | eapply le_sort_by; eassumption].
+Admitted  (*TODO:finish*).
+
+(* combines le_term_by and le_term_subst *)
+Lemma le_term_by' name l c : forall c' t e1 e2 s1 s2 t' e1' e2',
+    [:> !c' |- (name) !e1 = !e2 : !t] \in l ->
+    len_eq s1 c' ->
+    len_eq s2 c' ->                          
+    t' = t[/with_names_from c' s2/] ->
+    e1' = e1[/with_names_from c' s1/] ->
+    e2' = e2[/with_names_from c' s2/] ->
+    le_args l c c' s1 s2 ->
+    le_term l c t' e1' e2'.
+Proof using .
+  intros.
+  repeat (match goal with [eqH : _ = _ |- _] => rewrite eqH; clear eqH end).
+  eapply le_term_subst;[ | eapply le_term_by; eassumption].
+Admitted  (*TODO:finish*).
+
+Arguments le_term_by' name [l] {c} {c'} {t} {e1} {e2} {s1} {s2} {t'} {e1'} {e2'}.
+
+
+
+(* Justification for eliding typing guarantees in inductive for le*)
+Lemma le_sort_preserves_wf l c t1 t2
+  : wf_lang l -> wf_sort l c t1 -> le_sort l c t1 t2 -> wf_sort l c t2.
+Proof.
+  intros wfl wft.
+  elim.
+  {
+    
+    intros.
